{
 "cells": [
  {
   "cell_type": "raw",
   "id": "d466efc5-3aa9-429d-84ac-ea64fecc7d90",
   "metadata": {},
   "source": [
    "#1.1) 𝑇(𝑛) = 𝑇(𝑛 − 1) + 2, 𝑇(1) = 1\n",
    "================================================\n",
    "T(n) = T(n-1) + 2\n",
    "T(1) = 1\n",
    "T(n) = T(n-1) + 2 = [T(n-2) + 2] + 2 = T(n-2) + 2 + 2\n",
    "T(n) = T(n-2) + 2*2\n",
    "T(n) = T(n-2) + 2*2 = [T(n-3) + 2] + 2*2 = T(n-3) + 2 + 2*2\n",
    "T(n) = T(n-3) + 2*3\n",
    "Substituting Equations\n",
    "n → n-1\n",
    "T(n-1) = T(n-2) + 2\n",
    "T(n-2) = T(n-3) + 2\n",
    "T(n-3) = T(n-4) + 2\n",
    "T(n-4) = T(n-5) + 2\n",
    "T(n) = T(n-3) + 2*3 = [T(n-4) + 2] + 2*3 = T(n-4) + 2 + 2*3\n",
    "T(n) = T(n-4) + 2*4\n",
    "Do it one more time…\n",
    "T(n) = T(n-4) + 2*4\n",
    "So now rewrite these five equations and look for a pattern:\n",
    "T(n) = T(n-1) + 2*1 1st step of recursion\n",
    "T(n) = T(n-2) + 2*2 2nd step of recursion\n",
    "T(n) = T(n-3) + 2*3 3rd step of recursion\n",
    "T(n) = T(n-4) + 2*4 4th step of recursion\n",
    "T(n) = T(n-5) + 2*5 5th step of recursion\n",
    "Generalized recurrence relation at the kth step of the recursion:\n",
    "T(n) = T(n-k) + 2*k\n",
    "We want T(1). So we let n-k = 1. Solving for k, we get k = n - 1. Now plug back in.\n",
    "T(n) = T(n-k) + 2*k\n",
    "T(n) = T(1) + 2*(n-1), and we know T(1) = 1\n",
    "T(n) = 2*(n-1) = 2n-1\n",
    "We are done. Right side does not have any T(…)’s. This recurrence relation is now solved in its\n",
    "closed form, and it runs in O(n) time"
   ]
  },
  {
   "cell_type": "raw",
   "id": "a46c6001-32ea-45ad-87e9-794f9fc5645f",
   "metadata": {},
   "source": [
    "#2.SUBSTITUTION METHOD\n",
    "a.T(n) = T(n-1) + n\n",
    "= T(n-2) + (n-1) + n\n",
    "= T(n-3) + (n-2) + (n-1) + n\n",
    "= ... \n",
    "= T(1) + (2 + 3 + ... + n)\n",
    "= T(0) + (1 + 2 + ... + n)\n",
    "= T(0) +  n * (n+1) / 2\n",
    "= O(n ^ 2)"
   ]
  },
  {
   "cell_type": "raw",
   "id": "f65c1872-cf0c-471b-a0f2-5718762fcd3f",
   "metadata": {},
   "source": [
    "b.T(n)=2T(n/2)+n\n",
    "\n",
    "2\n",
    "\n",
    "Note that\n",
    "T(n)n=T(n/2)n/2+1\n",
    "\n",
    "Use substitution\n",
    "\n",
    "S(n)=T(2n)=2T(2n2)+2n=2T(2n−1)+2n=2S(n−1)+2n\n",
    "\n",
    "So you have to solve recursion\n",
    "\n",
    "S(n)=2S(n−1)+2n,\n",
    "\n",
    "or\n",
    "\n",
    "S(n)−2S(n−1)=2n.\n",
    "\n",
    "So,\n",
    "\n",
    "S(n−1)−2S(n−2)=2n−1\n",
    "\n",
    "and\n",
    "\n",
    "2S(n−1)−4S(n−2)=2n\n",
    "\n",
    "So,\n",
    "\n",
    "S(n)−2S(n−1)=2S(n−1)−4S(n−2)\n",
    "\n",
    "or\n",
    "\n",
    "S(n)−4S(n−1)+4S(n−1)=0.\n",
    "\n",
    "Characteristic equation for the recursion is\n",
    "\n",
    "x2−4x+4=0,\n",
    "\n",
    "or\n",
    "\n",
    "(x−2)2=0.\n",
    "\n",
    "This equation has troots x1=x2=2\n",
    ", so general solution for it is\n",
    "\n",
    "S(n)=C12n+C2n2n.\n",
    "\n",
    "At the end you turn back to T(n)\n",
    ".\n",
    "\n",
    "T(n)=S(lgn)=C1n+C2nlgn\n",
    "\n",
    "From the last equation you can conclude that\n",
    "\n",
    "T(n)=Θ(nlgn)"
   ]
  },
  {
   "cell_type": "raw",
   "id": "79a3bc55-f581-4f61-abbb-040e1019f7c0",
   "metadata": {},
   "source": [
    "c. T(n)=2T(n/2)+Θ(1)\n",
    "     =2T(n/2)+k\n",
    "     =2{2T(n/4)+k)+k\n",
    "     =4T(n/4)+3k\n",
    "     =...\n",
    "     =n.T(1)+(n-1)k\n",
    "     =n.k+(n-1)k\n",
    "     =2nk-k\n",
    "     =O(n)."
   ]
  },
  {
   "cell_type": "raw",
   "id": "e3236fa7-82fe-46ea-a1cc-d9cf597b1311",
   "metadata": {},
   "source": [
    "d.T(N) = T(N/2) + N              T(1)=0\n",
    "T(N/2) = T(N/4) + N/2\n",
    "T(N/4) = T(N/8) + N/4\n",
    "...\n",
    "T(2) = T(1) + 2\n",
    "\n",
    "T(N)= T(1) + N + N/2 + N/4"
   ]
  },
  {
   "cell_type": "markdown",
   "id": "638bb1c6-65e3-4e37-8105-319907dbfe79",
   "metadata": {},
   "source": [
    "#3a)T(n)=2T(n-1)+1\n",
    "T(0)=1\n",
    ". Then\n",
    "\n",
    "T(n)=2T(n−1)+n=4T(n−2)+2(n−1)+n=8T(n−3)+4(n−2)+2(n−1)+n⋮=2kT(n−k)+∑i=0k−12i(n−i)⋮=2nT(0)+∑i=0n−12i(n−i)=2n+n(2n−1)−\n",
    "∑i=0n−1i2i=2n+n(2n−1)−∑i=1n−1∑j=1i2i=2n+n(2n−1)−∑j=1n−1∑i=jn−12i=2n+n(2n−1)−∑j=1n−1(2n−2j)=2n+n(2n−1)−n2n+∑j=1n−12j=2n−n+2n−2=2n+1−n−2.\n",
    "This is Θ(2n)\n",
    ", but it’s not Θ(n2n)\n",
    ", because it’s not Ω(n2n)\n",
    ":\n",
    "limn→∞2n+1−n−2n2n=0.\n",
    "Share\n",
    "Cite\n",
    "Follow\n",
    "answered Jan 31, 2012 at 23:03\n",
    "Brian M. Scott's user avatar\n",
    "Brian M. Scott\n",
    "620k5858 gold badges789789 silver badges1.3k1.3k bronze badges\n",
    "Add a comment\n",
    "1\n",
    "\n",
    "Recall that Θ(n)\n",
    " denotes any sequence (R(n))\n",
    " such that there exists some finite and positive n0\n",
    ", c\n",
    " and C\n",
    ", such that cn⩽R(n)⩽Cn\n",
    " for every n⩾n0\n",
    ". Hence the hypothesis is that, for every n⩾n0\n",
    ",\n",
    "2T(n−1)+cn⩽T(n)⩽2T(n−1)+Cn.\n",
    "Equivalently, t(n)=2−nT(n)\n",
    " is such that, for every n⩾n0\n",
    ",\n",
    "t(n−1)+cn2−n⩽t(n)⩽t(n−1)+Cn2−n.\n",
    "Iterating this yields\n",
    "t(n0)+cs(n)⩽t(n)⩽t(n0)+Cs(n),s(n)=∑k=n0+1nk2−k.\n",
    "In particular, for every n⩾n0+1\n",
    ",\n",
    "t(n0)+cs∗⩽t(n)⩽t(n0)+Cs∗,s∗=(n0+1)2−n0,s∗=∑k=n0+1+∞k2−k.\n",
    "Assume for a moment that s∗\n",
    " is finite. Then a2n≤T(n)⩽A2n\n",
    " for every n⩾n0+1\n",
    ", with a=t(n0)+cs∗\n",
    " and A=t(n0)+Cs∗\n",
    ", both positive and finite, hence T(n)=Θ(2n)\n",
    ".\n",
    "\n",
    "Finally, s∗\n",
    " is finite if and only if s0\n",
    " is, where\n",
    "s0=∑k=0+∞k2−k.\n",
    "Recall that s0=12σ′(12)\n",
    " where, for every |x|<1\n",
    ",\n",
    "σ(x)=∑k=0+∞xk=(1−x)−1,\n",
    "hence σ′(x)=(1−x)−2\n",
    " and s0=2\n",
    " is finite.\n",
    "\n",
    "Share\n",
    "Cite\n",
    "Follow\n",
    "answered Jan 31, 2012 at 22:52\n",
    "Did's user avatar\n",
    "Did\n",
    "281k2727 gold badges310310 silver badges590590 bronze badges\n",
    "Add a comment\n",
    "0\n",
    "\n",
    "OK, I've been very confused by this notation, but are you sure that the answer is Θ(n⋅2n)\n",
    "?\n",
    "\n",
    "Your tree analysis is correct: at the first step, you add Θ(n)\n",
    ", at the next one, you add 2Θ(n−1)\n",
    ", at the next one 4Θ(n−2)\n",
    ", etc. In other words, at the i\n",
    "-th step, you add 2iΘ(n−i)\n",
    ". Because you need to add all the steps, the actual sum is then\n",
    "T(n)=∑i=0n2iΘ(n−i)\n",
    "Now, since Θ(n)\n",
    " means \"a function doing n\n",
    " steps of computation\", you can rewrite Θ(n−i)\n",
    " as Θ(n)−Θ(i)\n",
    ". The sum becomes\n",
    "T(n)=∑i=0n2iΘ(n)−2iΘ(i)=∑i=0n2iΘ(n)−∑i=0n2iΘ(i)\n",
    "If we pull Θ(n)\n",
    " out of the sum, we can use the fact that ∑ni=02i=2n+1−1\n",
    ". Moreover, we can use the fact that ∑ni=0i⋅2i=2(n⋅2n−2n+1)\n",
    ". The sum then becomes:\n",
    "T(n)=n∗(2n+1−1)−2(n⋅2n−2n+1)=−n+2n+1−2\n",
    "So I would conclude that T(n)=Θ(2n)\n",
    ".\n",
    "\n",
    "Actually, according to Wolfram Alpha, we have t(n)=−n+3⋅2n−2\n",
    ".\n",
    "\n",
    "So either I also made a mistake in the calculation (which is obviously possible), or the answer is indeed Θ(2n)\n",
    ", as you found yourself."
   ]
  },
  {
   "cell_type": "markdown",
   "id": "a2bd6a05-f5c1-433f-8954-b1799ab0ee09",
   "metadata": {},
   "source": [
    "#3.b)T(n)=2T(n/2)+n\n",
    " n/20 -→ n/21 -→ n/22 -→ ……… -→ n/2k\n",
    "\n",
    "Size of problem at last level = n/2k\n",
    "\n",
    " At last level size of problem becomes 1\n",
    "\n",
    " n/2k = 1\n",
    "\n",
    " 2k = n\n",
    "\n",
    "  k = log2(n)   \n",
    "\n",
    "Total no of levels  in recursive tree = k +1 = log2(n) + 1\n",
    "\n",
    "Step 3: Count total number of nodes in the last level and calculate cost of last level\n",
    " No. of nodes at level 0 = 20 = 1\n",
    "\n",
    "  No. of nodes at level 1 = 21 = 2\n",
    "\n",
    " ………………………………………………………\n",
    "\n",
    "No. of nodes at the (k+1)th level (or last level) = 2k = 2log2(n) = nlog2(2) = n\n",
    "\n",
    " Cost of sub problems at level last level = n x Θ(1) = Θ(n)\n",
    "\n",
    "Step 4: Sum up the cost all the levels in recursive tree  \n",
    "   T(n) = c + 2c + 4c + —- ((no. of levels-1) times) + last level cost\n",
    "\n",
    " = c + 2c + 4c + —- (log2(n) times) + Θ(n)\n",
    "\n",
    " = c(1 + 2 + 4 + —- (log2(n) times)) + Θ(n)\n",
    "\n",
    " 1 + 2 + 4 + —– (log2(n) times) –> 20 + 21 + 22 + —– (log2(n) times) –> Geometric Progression(G.P.)\n",
    "\n",
    "Using GP Sum Formula, we get the sum of the series as n\n",
    "\n",
    "= c(n) + Θ(n)"
   ]
  },
  {
   "cell_type": "code",
   "execution_count": null,
   "id": "ae45c6be-35fe-4504-a582-f4686a8907e7",
   "metadata": {},
   "outputs": [],
   "source": [
    "                 ..........THANKYOU.........."
   ]
  }
 ],
 "metadata": {
  "kernelspec": {
   "display_name": "Python 3 (ipykernel)",
   "language": "python",
   "name": "python3"
  },
  "language_info": {
   "codemirror_mode": {
    "name": "ipython",
    "version": 3
   },
   "file_extension": ".py",
   "mimetype": "text/x-python",
   "name": "python",
   "nbconvert_exporter": "python",
   "pygments_lexer": "ipython3",
   "version": "3.10.8"
  }
 },
 "nbformat": 4,
 "nbformat_minor": 5
}
